re-structuring proof scripts in Ackermann sub-directory

theories/ordinals/Ackermann/codeFreeVar.v
@@ -8,6 +8,7 @@ Require Import folProp.
 Require Import code.
 Require Import Compat815.
 
+Import LispAbbreviations.
 Section Code_Free_Vars.
 
 Variable L : Language.
@@ -36,760 +37,612 @@ Definition codeFreeVarTermTerms : nat -> nat :=
   evalStrongRec 0
     (fun t recs : nat =>
      cPair
-       (switchPR (cPairPi1 t) (cPairPi2 (codeNth (t - S (cPairPi2 t)) recs))
-          (S (cPair (cPairPi2 t) 0)))
+       (switchPR (car t) (cdr (codeNth (t - S (cdr t)) recs))
+          (S (cPair (cdr t) 0)))
        (switchPR t
-          (codeApp (cPairPi1 (codeNth (t - S (cPairPi1 (pred t))) recs))
-             (cPairPi2 (codeNth (t - S (cPairPi2 (pred t))) recs))) 0)).
+          (codeApp (car (codeNth (t - S (car (pred t))) recs))
+             (cdr (codeNth (t - S (cdr (pred t))) recs))) 0)).
 
 Definition codeFreeVarTerm (t : nat) : nat :=
-  cPairPi1 (codeFreeVarTermTerms t).
+  car (codeFreeVarTermTerms t).
 
 Definition codeFreeVarTerms (t : nat) : nat :=
-  cPairPi2 (codeFreeVarTermTerms t).
+  cdr (codeFreeVarTermTerms t).
 
 Lemma codeFreeVarTermCorrect :
  forall t : Term,
  codeFreeVarTerm (codeTerm L codeF t) = codeList (freeVarTerm L t).
 Proof.
-intros.
-elim t using
- Term_Terms_ind
+ intros t; elim t using  Term_Terms_ind
   with
     (P0 := fun (n : nat) (ts : fol.Terms L n) =>
            codeFreeVarTerms (codeTerms L codeF n ts) =
            codeList (freeVarTerms L n ts)); intros.
-simpl in |- *.
-unfold codeTerm in |- *.
-unfold codeFreeVarTerm in |- *.
-unfold codeFreeVarTermTerms in |- *.
-unfold evalStrongRec in |- *.
-simpl in |- *.
-repeat rewrite cPairProjections1 || rewrite cPairProjections2.
-simpl in |- *.
-reflexivity.
-unfold freeVarTerm in |- *.
-fold (freeVarTerms L (arity L (inr (Relations L) f)) t0) in |- *.
-rewrite <- H.
-clear H.
-unfold codeTerm in |- *.
-fold (codeTerms L codeF (arity L (inr (Relations L) f)) t0) in |- *.
-generalize (codeTerms L codeF (arity L (inr (Relations L) f)) t0).
-intros.
-unfold codeFreeVarTerm in |- *.
-unfold codeFreeVarTermTerms in |- *.
-set
- (g :=
-  fun t1 recs : nat =>
-  cPair
-    (switchPR (cPairPi1 t1) (cPairPi2 (codeNth (t1 - S (cPairPi2 t1)) recs))
-       (S (cPair (cPairPi2 t1) 0)))
-    (switchPR t1
-       (codeApp (cPairPi1 (codeNth (t1 - S (cPairPi1 (pred t1))) recs))
-          (cPairPi2 (codeNth (t1 - S (cPairPi2 (pred t1))) recs))) 0)) 
- in *.
-unfold evalStrongRec in |- *.
-unfold evalComposeFunc in |- *.
-unfold evalOneParamList in |- *.
-rewrite computeEvalStrongRecHelp.
-unfold compose2 in |- *.
-unfold evalComposeFunc in |- *.
-unfold g at 1 in |- *.
-repeat rewrite cPairProjections1 || rewrite cPairProjections2.
-rewrite (evalStrongRecHelp1 g (cPair (S (codeF f)) n) n).
-simpl in |- *.
-repeat rewrite cPairProjections1 || rewrite cPairProjections2.
-unfold codeFreeVarTerms in |- *.
-unfold codeFreeVarTermTerms in |- *.
-fold g in |- *.
-reflexivity.
-apply cPairLt2.
-simpl in |- *.
-unfold codeTerms in |- *.
-unfold codeFreeVarTerms in |- *.
-unfold codeFreeVarTermTerms in |- *.
-unfold evalStrongRec in |- *.
-simpl in |- *.
-repeat rewrite cPairProjections1 || rewrite cPairProjections2.
-reflexivity.
-unfold freeVarTerms in |- *.
-fold (freeVarTerm L t0) in |- *.
-fold (freeVarTerms L n t1) in |- *.
-rewrite <- codeAppCorrect.
-rewrite <- H.
-rewrite <- H0.
-clear H H0.
-unfold codeTerms in |- *.
-fold (codeTerm L codeF t0) in |- *.
-fold (codeTerms L codeF n t1) in |- *.
-generalize (codeTerm L codeF t0) (codeTerms L codeF n t1).
-clear t0 t1.
-intros.
-unfold codeFreeVarTerms at 1 in |- *.
-unfold codeFreeVarTermTerms in |- *.
-unfold evalStrongRec in |- *.
-set
- (g :=
-  fun t0 recs : nat =>
-  cPair
-    (switchPR (cPairPi1 t0) (cPairPi2 (codeNth (t0 - S (cPairPi2 t0)) recs))
-       (S (cPair (cPairPi2 t0) 0)))
-    (switchPR t0
-       (codeApp (cPairPi1 (codeNth (t0 - S (cPairPi1 (pred t0))) recs))
-          (cPairPi2 (codeNth (t0 - S (cPairPi2 (pred t0))) recs))) 0)) 
- in *.
-unfold evalComposeFunc in |- *.
-unfold evalOneParamList in |- *.
-rewrite computeEvalStrongRecHelp.
-unfold compose2 in |- *.
-unfold evalComposeFunc in |- *.
-unfold g at 1 in |- *.
-rewrite
- (evalStrongRecHelp1 g (S (cPair n0 n1)) (cPairPi1 (pred (S (cPair n0 n1)))))
- .
-rewrite
- (evalStrongRecHelp1 g (S (cPair n0 n1)) (cPairPi2 (pred (S (cPair n0 n1)))))
- .
-simpl in |- *.
-repeat rewrite cPairProjections1 || rewrite cPairProjections2.
-reflexivity.
-simpl in |- *.
-rewrite cPairProjections2.
-apply Compat815.le_lt_n_Sm.
-apply cPairLe2.
-simpl in |- *.
-rewrite cPairProjections1.
-apply Compat815.le_lt_n_Sm.
-apply cPairLe1.
+ - simpl; unfold codeTerm, codeFreeVarTerm, codeFreeVarTermTerms,
+     evalStrongRec in |- *.
+   simpl; repeat rewrite cPairProjections1 || rewrite cPairProjections2.
+   simpl; reflexivity.
+ - unfold freeVarTerm; fold (freeVarTerms L (arity L (inr (Relations L) f)) t0).
+   rewrite <- H; clear H.
+   unfold codeTerm; fold (codeTerms L codeF (arity L (inr (Relations L) f)) t0).
+   generalize (codeTerms L codeF (arity L (inr (Relations L) f)) t0).
+   intros n; unfold codeFreeVarTerm, codeFreeVarTermTerms.
+   set
+     (g := fun t1 recs : nat =>
+             cPair
+               (switchPR (car t1) (cdr 
+                                          (codeNth (t1 - S (cdr t1)) recs))
+                  (S (cPair (cdr t1) 0)))
+               (switchPR t1
+                  (codeApp (car (codeNth 
+                                        (t1 - S (car (pred t1))) recs))
+                     (cdr (codeNth (t1 - S (cdr (pred t1))) recs))) 0))      in *.
+   unfold evalStrongRec, evalComposeFunc, evalOneParamList.
+   rewrite computeEvalStrongRecHelp.
+   unfold compose2 in |- *.
+   unfold evalComposeFunc in |- *.
+   unfold g at 1 in |- *.
+   repeat rewrite cPairProjections1 || rewrite cPairProjections2.
+   rewrite (evalStrongRecHelp1 g (cPair (S (codeF f)) n) n).
+   + simpl; repeat rewrite cPairProjections1 || rewrite cPairProjections2.
+     unfold codeFreeVarTerms; unfold codeFreeVarTermTerms.
+     fold g; reflexivity.
+   + apply cPairLt2.
+ - simpl; unfold codeTerms, codeFreeVarTerms, codeFreeVarTermTerms.
+   unfold evalStrongRec; simpl; 
+     repeat rewrite cPairProjections1 || rewrite cPairProjections2.
+   reflexivity.
+ - unfold freeVarTerms; fold (freeVarTerm L t0);
+     fold (freeVarTerms L n t1); rewrite <- codeAppCorrect.
+   rewrite <- H; rewrite <- H0; clear H H0.
+   unfold codeTerms.
+   fold (codeTerm L codeF t0); fold (codeTerms L codeF n t1).
+   generalize (codeTerm L codeF t0) (codeTerms L codeF n t1).
+   clear t0 t1.
+   intros n0 n1; unfold codeFreeVarTerms at 1 in |- *.
+   unfold codeFreeVarTermTerms in |- *.
+   unfold evalStrongRec in |- *.
+   set
+     (g :=
+        fun t0 recs : nat =>
+          cPair
+            (switchPR (car t0) 
+               (cdr (codeNth (t0 - S (cdr t0)) recs))
+               (S (cPair (cdr t0) 0)))
+            (switchPR t0
+               (codeApp (car (codeNth (t0 - S (car (pred t0))) recs))
+                  (cdr (codeNth (t0 - S (cdr (pred t0))) recs))) 0)) 
+     in *.
+   unfold evalComposeFunc, evalOneParamList. 
+   rewrite computeEvalStrongRecHelp.
+   unfold compose2, evalComposeFunc; unfold g at 1.
+   rewrite
+     (evalStrongRecHelp1 g (S (cPair n0 n1))
+        (car (pred (S (cPair n0 n1))))).
+   + rewrite
+       (evalStrongRecHelp1 g (S (cPair n0 n1)) 
+          (cdr (pred (S (cPair n0 n1))))).
+     simpl; repeat rewrite cPairProjections1 || rewrite cPairProjections2.
+     reflexivity.
+     simpl; rewrite cPairProjections2.
+     apply Compat815.le_lt_n_Sm.
+     apply cPairLe2.
+   + simpl; rewrite cPairProjections1.
+     apply Compat815.le_lt_n_Sm.
+     apply cPairLe1.
 Qed.
 
-Lemma codeFreeVarTermsCorrect :
- forall (n : nat) (ts : Terms n),
+Lemma codeFreeVarTermsCorrect (n : nat) (ts : Terms n):
  codeFreeVarTerms (codeTerms L codeF n ts) = codeList (freeVarTerms L n ts).
 Proof.
-intros.
-induction ts as [| n t ts Hrects].
-simpl in |- *.
-unfold codeTerms in |- *.
-unfold codeFreeVarTerms in |- *.
-unfold codeFreeVarTermTerms in |- *.
-unfold evalStrongRec in |- *.
-simpl in |- *.
-repeat rewrite cPairProjections1 || rewrite cPairProjections2.
-reflexivity.
-unfold freeVarTerms in |- *.
-fold (freeVarTerm L t) in |- *.
-fold (freeVarTerms L n ts) in |- *.
-rewrite <- codeAppCorrect.
-rewrite <- Hrects.
-rewrite <- codeFreeVarTermCorrect.
-clear Hrects.
-unfold codeTerms in |- *.
-fold (codeTerm L codeF t) in |- *.
-fold (codeTerms L codeF n ts) in |- *.
-generalize (codeTerm L codeF t) (codeTerms L codeF n ts).
-clear t ts.
-intros.
-unfold codeFreeVarTerms at 1 in |- *.
-unfold codeFreeVarTermTerms in |- *.
-unfold evalStrongRec in |- *.
-set
- (g :=
-  fun t0 recs : nat =>
-  cPair
-    (switchPR (cPairPi1 t0) (cPairPi2 (codeNth (t0 - S (cPairPi2 t0)) recs))
-       (S (cPair (cPairPi2 t0) 0)))
-    (switchPR t0
-       (codeApp (cPairPi1 (codeNth (t0 - S (cPairPi1 (pred t0))) recs))
-          (cPairPi2 (codeNth (t0 - S (cPairPi2 (pred t0))) recs))) 0)) 
- in *.
-unfold evalComposeFunc in |- *.
-unfold evalOneParamList in |- *.
-rewrite computeEvalStrongRecHelp.
-unfold compose2 in |- *.
-unfold evalComposeFunc in |- *.
-unfold g at 1 in |- *.
-rewrite
- (evalStrongRecHelp1 g (S (cPair n0 n1)) (cPairPi1 (pred (S (cPair n0 n1)))))
- .
-rewrite
- (evalStrongRecHelp1 g (S (cPair n0 n1)) (cPairPi2 (pred (S (cPair n0 n1)))))
- .
-simpl in |- *.
-repeat rewrite cPairProjections1 || rewrite cPairProjections2.
-reflexivity.
-simpl in |- *.
-rewrite cPairProjections2.
-apply Compat815.le_lt_n_Sm.
-apply cPairLe2.
-simpl in |- *.
-rewrite cPairProjections1.
-apply Nat.lt_succ_r.
-apply cPairLe1.
+  induction ts as [| n t ts Hrects].
+  - simpl; unfold codeTerms, codeFreeVarTerms, codeFreeVarTermTerms.
+    unfold evalStrongRec; simpl.
+    repeat rewrite cPairProjections1 || rewrite cPairProjections2.
+    reflexivity.
+  - unfold freeVarTerms; fold (freeVarTerm L t); fold (freeVarTerms L n ts).
+    rewrite <- codeAppCorrect.
+    rewrite <- Hrects.
+    rewrite <- codeFreeVarTermCorrect; clear Hrects.
+    unfold codeTerms; fold (codeTerm L codeF t); fold (codeTerms L codeF n ts).
+    generalize (codeTerm L codeF t) (codeTerms L codeF n ts).
+    clear t ts.
+    intros n0 n1;
+      unfold codeFreeVarTerms at 1; unfold codeFreeVarTermTerms.
+    unfold evalStrongRec in |- *.
+    set
+      (g :=
+         fun t0 recs : nat =>
+           cPair
+             (switchPR (car t0)
+                (cdr (codeNth (t0 - S (cdr t0)) recs))
+                (S (cPair (cdr t0) 0)))
+             (switchPR t0
+                (codeApp (car (codeNth (t0 - S (car (pred t0))) recs))
+                   (cdr (codeNth (t0 - S (cdr (pred t0))) recs))) 0)). 
+    unfold evalComposeFunc, evalOneParamList.
+    rewrite computeEvalStrongRecHelp.
+    unfold compose2, evalComposeFunc; unfold g at 1.
+    + rewrite
+        (evalStrongRecHelp1 g (S (cPair n0 n1)) 
+           (car (pred (S (cPair n0 n1))))).
+      * rewrite  (evalStrongRecHelp1 g (S (cPair n0 n1)) 
+                    (cdr (pred (S (cPair n0 n1))))).
+        -- simpl; repeat rewrite cPairProjections1 || rewrite cPairProjections2.
+           reflexivity.
+        -- simpl; rewrite cPairProjections2.
+           apply Compat815.le_lt_n_Sm.
+           apply cPairLe2.
+      * simpl; rewrite cPairProjections1.
+        apply Nat.lt_succ_r.
+        apply cPairLe1.
 Qed.
 
 Lemma codeFreeVarTermTermsIsPR : isPR 1 codeFreeVarTermTerms.
 Proof.
-intros.
-unfold codeFreeVarTermTerms in |- *.
-apply evalStrongRecIsPR.
-apply
- compose2_2IsPR
-  with
+  unfold codeFreeVarTermTerms; apply evalStrongRecIsPR.
+  apply
+    compose2_2IsPR
+    with
     (f := fun t recs : nat =>
-          switchPR (cPairPi1 t)
-            (cPairPi2 (codeNth (t - S (cPairPi2 t)) recs))
-            (S (cPair (cPairPi2 t) 0)))
+            switchPR (car t)
+              (cdr (codeNth (t - S (cdr t)) recs))
+              (S (cPair (cdr t) 0)))
     (g := fun t recs : nat =>
-          switchPR t
-            (codeApp (cPairPi1 (codeNth (t - S (cPairPi1 (pred t))) recs))
-               (cPairPi2 (codeNth (t - S (cPairPi2 (pred t))) recs))) 0).
-apply
- compose2_3IsPR
-  with
-    (f1 := fun t recs : nat => cPairPi1 t)
-    (f2 := fun t recs : nat => cPairPi2 (codeNth (t - S (cPairPi2 t)) recs))
-    (f3 := fun t recs : nat => S (cPair (cPairPi2 t) 0)).
-apply filter10IsPR.
-apply cPairPi1IsPR.
-apply
- compose2_1IsPR
-  with (f := fun t recs : nat => codeNth (t - S (cPairPi2 t)) recs).
-apply
- compose2_2IsPR
-  with
-    (f := fun t recs : nat => t - S (cPairPi2 t))
-    (g := fun t recs : nat => recs).
-apply filter10IsPR with (g := fun t : nat => t - S (cPairPi2 t)).
-apply
- compose1_2IsPR
-  with (f := fun t : nat => t) (f' := fun t : nat => S (cPairPi2 t)).
-apply idIsPR.
-apply compose1_1IsPR.
-apply cPairPi2IsPR.
-apply succIsPR.
-apply minusIsPR.
-apply pi2_2IsPR.
-apply codeNthIsPR.
-apply cPairPi2IsPR.
-apply filter10IsPR with (g := fun t : nat => S (cPair (cPairPi2 t) 0)).
-apply compose1_1IsPR with (f := fun t : nat => cPair (cPairPi2 t) 0).
-apply compose1_2IsPR with (f := cPairPi2) (f' := fun _ : nat => 0).
-apply cPairPi2IsPR.
-apply const1_NIsPR.
-apply cPairIsPR.
-apply succIsPR.
-apply switchIsPR.
-apply
- compose2_3IsPR
-  with
-    (f1 := fun t recs : nat => t)
-    (f2 := fun t recs : nat =>
-           codeApp (cPairPi1 (codeNth (t - S (cPairPi1 (pred t))) recs))
-             (cPairPi2 (codeNth (t - S (cPairPi2 (pred t))) recs)))
-    (f3 := fun t recs : nat => 0).
-apply pi1_2IsPR.
-apply
- compose2_2IsPR
-  with
-    (f := fun t recs : nat =>
-          cPairPi1 (codeNth (t - S (cPairPi1 (pred t))) recs))
-    (g := fun t recs : nat =>
-          cPairPi2 (codeNth (t - S (cPairPi2 (pred t))) recs)).
-apply
- compose2_1IsPR
-  with (f := fun t recs : nat => codeNth (t - S (cPairPi1 (pred t))) recs).
-apply
- compose2_2IsPR
-  with
-    (f := fun t recs : nat => t - S (cPairPi1 (pred t)))
-    (g := fun t recs : nat => recs).
-apply filter10IsPR with (g := fun t : nat => t - S (cPairPi1 (pred t))).
-apply
- compose1_2IsPR
-  with (f := fun t : nat => t) (f' := fun t : nat => S (cPairPi1 (pred t))).
-apply idIsPR.
-apply compose1_1IsPR with (f := fun t : nat => cPairPi1 (pred t)).
-apply compose1_1IsPR.
-apply predIsPR.
-apply cPairPi1IsPR.
-apply succIsPR.
-apply minusIsPR.
-apply pi2_2IsPR.
-apply codeNthIsPR.
-apply cPairPi1IsPR.
-apply
- compose2_1IsPR
-  with (f := fun t recs : nat => codeNth (t - S (cPairPi2 (pred t))) recs).
-apply
- compose2_2IsPR
-  with
-    (f := fun t recs : nat => t - S (cPairPi2 (pred t)))
-    (g := fun t recs : nat => recs).
-apply filter10IsPR with (g := fun t : nat => t - S (cPairPi2 (pred t))).
-apply
- compose1_2IsPR
-  with (f := fun t : nat => t) (f' := fun t : nat => S (cPairPi2 (pred t))).
-apply idIsPR.
-apply compose1_1IsPR with (f := fun t : nat => cPairPi2 (pred t)).
-apply compose1_1IsPR.
-apply predIsPR.
-apply cPairPi2IsPR.
-apply succIsPR.
-apply minusIsPR.
-apply pi2_2IsPR.
-apply codeNthIsPR.
-apply cPairPi2IsPR.
-apply codeAppIsPR.
-exists (composeFunc 2 0 (PRnil _) zeroFunc).
-simpl in |- *.
-auto.
-apply switchIsPR.
-apply cPairIsPR.
+            switchPR t
+              (codeApp (car (codeNth (t - S (car (pred t))) recs))
+                 (cdr (codeNth (t - S (cdr (pred t))) recs))) 0).
+  - apply compose2_3IsPR with
+      (f1 := fun t recs : nat => car t)
+      (f2 := fun t recs : nat => cdr (codeNth (t - S (cdr t)) recs))
+      (f3 := fun t recs : nat => S (cPair (cdr t) 0)).
+    + apply filter10IsPR.
+      apply cPairPi1IsPR.
+    + apply compose2_1IsPR with 
+        (f := fun t recs : nat => codeNth (t - S (cdr t)) recs).
+      * apply compose2_2IsPR with
+          (f := fun t recs : nat => t - S (cdr t))
+          (g := fun t recs : nat => recs).
+        -- apply filter10IsPR with 
+             (g := fun t : nat => t - S (cdr t)).
+           apply compose1_2IsPR with
+             (f := fun t : nat => t) (f' := fun t : nat => S (cdr t)).
+           ++ apply idIsPR.
+           ++ apply compose1_1IsPR.
+              apply cPairPi2IsPR.
+              apply succIsPR.
+           ++ apply minusIsPR.
+        -- apply pi2_2IsPR.
+        -- apply codeNthIsPR.
+      * apply cPairPi2IsPR.
+    + apply filter10IsPR with (g := fun t : nat => S (cPair (cdr t) 0)).
+      apply compose1_1IsPR with (f := fun t : nat => cPair (cdr t) 0).
+      * apply compose1_2IsPR with (f := cPairPi2) (f' := fun _ : nat => 0).
+        -- apply cPairPi2IsPR.
+        -- apply const1_NIsPR.
+        -- apply cPairIsPR.
+      * apply succIsPR.
+    + apply switchIsPR.
+  - apply compose2_3IsPR with
+      (f1 := fun t recs : nat => t)
+      (f2 := fun t recs : nat =>
+               codeApp (car (codeNth (t - S (car (pred t))) recs))
+                 (cdr (codeNth (t - S (cdr (pred t))) recs)))
+      (f3 := fun t recs : nat => 0).
+    + apply pi1_2IsPR.
+    + apply compose2_2IsPR with
+        (f := fun t recs : nat =>
+                car (codeNth (t - S (car (pred t))) recs))
+        (g := fun t recs : nat =>
+                cdr (codeNth (t - S (cdr (pred t))) recs)).
+      * apply compose2_1IsPR with 
+          (f := fun t recs : nat => codeNth (t - S (car (pred t))) recs).
+        -- apply compose2_2IsPR with
+             (f := fun t recs : nat => t - S (car (pred t)))
+             (g := fun t recs : nat => recs).
+           ++ apply filter10IsPR with
+                (g := fun t : nat => t - S (car (pred t))).
+              apply compose1_2IsPR with 
+                (f := fun t : nat => t)
+                (f' := fun t : nat => S (car (pred t))).
+              ** apply idIsPR.
+              ** apply compose1_1IsPR with 
+                   (f := fun t : nat => car (pred t)).
+                 apply compose1_1IsPR.
+                 apply predIsPR.
+                 apply cPairPi1IsPR.
+                 apply succIsPR.
+              ** apply minusIsPR.
+           ++ apply pi2_2IsPR.
+           ++ apply codeNthIsPR.
+        -- apply cPairPi1IsPR.
+      * apply compose2_1IsPR with 
+          (f := fun t recs : nat => codeNth (t - S (cdr (pred t))) recs).
+        -- apply compose2_2IsPR with
+             (f := fun t recs : nat => t - S (cdr (pred t)))
+             (g := fun t recs : nat => recs).
+           ++ apply filter10IsPR with 
+             (g := fun t : nat => t - S (cdr (pred t))).
+              apply compose1_2IsPR with 
+                (f := fun t : nat => t) 
+                (f' := fun t : nat => S (cdr (pred t))).
+              ** apply idIsPR.
+              ** apply compose1_1IsPR with 
+                   (f := fun t : nat => cdr (pred t)).
+                 apply compose1_1IsPR.
+                 apply predIsPR.
+                 apply cPairPi2IsPR.
+                 apply succIsPR.
+              ** apply minusIsPR.
+           ++ apply pi2_2IsPR.
+           ++ apply codeNthIsPR.
+        -- apply cPairPi2IsPR.
+      * apply codeAppIsPR.
+    + exists (composeFunc 2 0 (PRnil _) zeroFunc).
+      simpl; auto.
+    + apply switchIsPR.
+  - apply cPairIsPR.
 Qed.
 
 Lemma codeFreeVarTermIsPR : isPR 1 codeFreeVarTerm.
 Proof.
-unfold codeFreeVarTerm in |- *.
-apply compose1_1IsPR.
-apply codeFreeVarTermTermsIsPR.
-apply cPairPi1IsPR.
+  unfold codeFreeVarTerm; apply compose1_1IsPR.
+  - apply codeFreeVarTermTermsIsPR.
+  - apply cPairPi1IsPR.
 Qed.
 
 Lemma codeFreeVarTermsIsPR : isPR 1 codeFreeVarTerms.
 Proof.
-unfold codeFreeVarTerms in |- *.
-apply compose1_1IsPR.
-apply codeFreeVarTermTermsIsPR.
-apply cPairPi2IsPR.
+  unfold codeFreeVarTerms; apply compose1_1IsPR.
+  - apply codeFreeVarTermTermsIsPR.
+  - apply cPairPi2IsPR.
 Qed.
 
 Definition codeFreeVarFormula : nat -> nat :=
   evalStrongRec 0
     (fun f recs : nat =>
-     switchPR (cPairPi1 f)
-       (switchPR (pred (cPairPi1 f))
-          (switchPR (pred (pred (cPairPi1 f)))
-             (switchPR (pred (pred (pred (cPairPi1 f))))
-                (codeFreeVarTerms (cPairPi2 f))
-                (codeListRemove (cPairPi1 (cPairPi2 f))
-                   (codeNth (f - S (cPairPi2 (cPairPi2 f))) recs)))
-             (codeNth (f - S (cPairPi2 f)) recs))
-          (codeApp (codeNth (f - S (cPairPi1 (cPairPi2 f))) recs)
-             (codeNth (f - S (cPairPi2 (cPairPi2 f))) recs)))
-       (codeApp (codeFreeVarTerm (cPairPi1 (cPairPi2 f)))
-          (codeFreeVarTerm (cPairPi2 (cPairPi2 f))))).
+     switchPR (car f)
+       (switchPR (pred (car f))
+          (switchPR (pred (pred (car f)))
+             (switchPR (pred (pred (pred (car f))))
+                (codeFreeVarTerms (cdr f))
+                (codeListRemove (cadr f)
+                   (codeNth (f - S (cddr f)) recs)))
+             (codeNth (f - S (cdr f)) recs))
+          (codeApp (codeNth (f - S (cadr  f)) recs)
+             (codeNth (f - S (cddr f)) recs)))
+       (codeApp (codeFreeVarTerm (cadr f))
+          (codeFreeVarTerm (cddr f)))).
 
-Lemma codeFreeVarFormulaCorrect :
- forall f : Formula,
- codeFreeVarFormula (codeFormula L codeF codeR f) =
- codeList (freeVarFormula L f).
+Lemma codeFreeVarFormulaCorrect (f : Formula) :
+  codeFreeVarFormula (codeFormula L codeF codeR f) =
+    codeList (freeVarFormula L f).
 Proof.
-intros.
-set
- (g :=
-  fun f recs : nat =>
-  switchPR (cPairPi1 f)
-    (switchPR (pred (cPairPi1 f))
-       (switchPR (pred (pred (cPairPi1 f)))
-          (switchPR (pred (pred (pred (cPairPi1 f))))
-             (codeFreeVarTerms (cPairPi2 f))
-             (codeListRemove (cPairPi1 (cPairPi2 f))
-                (codeNth (f - S (cPairPi2 (cPairPi2 f))) recs)))
-          (codeNth (f - S (cPairPi2 f)) recs))
-       (codeApp (codeNth (f - S (cPairPi1 (cPairPi2 f))) recs)
-          (codeNth (f - S (cPairPi2 (cPairPi2 f))) recs)))
-    (codeApp (codeFreeVarTerm (cPairPi1 (cPairPi2 f)))
-       (codeFreeVarTerm (cPairPi2 (cPairPi2 f))))) 
- in *.
-induction f as [t t0| r t| f1 Hrecf1 f0 Hrecf0| f Hrecf| n f Hrecf].
-simpl in |- *.
-rewrite <- codeAppCorrect.
-repeat rewrite <- codeFreeVarTermCorrect.
-generalize (codeTerm L codeF t) (codeTerm L codeF t0).
-clear t t0.
-intros.
-unfold codeFreeVarFormula in |- *.
-unfold evalStrongRec in |- *.
-simpl in |- *.
-repeat rewrite cPairProjections1 || rewrite cPairProjections2.
-simpl in |- *.
-reflexivity.
-simpl in |- *.
-rewrite <- codeFreeVarTermsCorrect.
-generalize (codeTerms L codeF (arity L (inl (Functions L) r)) t).
-clear t.
-intros.
-unfold codeFreeVarFormula in |- *.
-unfold evalStrongRec in |- *.
-unfold evalStrongRecHelp in |- *.
-unfold evalComposeFunc in |- *.
-unfold evalOneParamList in |- *.
-unfold evalPrimRecFunc in |- *.
-repeat rewrite cPairProjections1 || rewrite cPairProjections2.
-simpl in |- *.
-repeat rewrite cPairProjections1 || rewrite cPairProjections2.
-reflexivity.
-simpl in |- *.
-rewrite <- codeAppCorrect.
-rewrite <- Hrecf1.
-rewrite <- Hrecf0.
-clear Hrecf0 Hrecf1.
-unfold codeFreeVarFormula in |- *.
-fold g in |- *.
-unfold evalStrongRec in |- *.
-unfold evalComposeFunc in |- *.
-unfold evalOneParamList in |- *.
-rewrite computeEvalStrongRecHelp.
-simpl in |- *.
-repeat rewrite cPairProjections1 || rewrite cPairProjections2.
-unfold g at 1 in |- *.
-repeat rewrite cPairProjections1 || rewrite cPairProjections2.
-rewrite
- (evalStrongRecHelp1 g
-    (cPair 1
-       (cPair (codeFormula L codeF codeR f1) (codeFormula L codeF codeR f0)))
-    (codeFormula L codeF codeR f1)).
-rewrite
- (evalStrongRecHelp1 g
-    (cPair 1
-       (cPair (codeFormula L codeF codeR f1) (codeFormula L codeF codeR f0)))
-    (codeFormula L codeF codeR f0)).
-simpl in |- *.
-unfold evalStrongRec in |- *.
-unfold evalComposeFunc in |- *.
-unfold evalOneParamList in |- *.
-simpl in |- *.
-repeat rewrite cPairProjections1 || rewrite cPairProjections2.
-reflexivity.
-eapply Nat.lt_le_trans.
-apply cPairLt2.
-apply cPairLe3.
-apply le_n.
-apply cPairLe2.
-eapply Nat.lt_le_trans.
-apply cPairLt2.
-apply cPairLe3.
-apply le_n.
-apply cPairLe1.
-simpl in |- *.
-rewrite <- Hrecf.
-clear Hrecf.
-generalize (codeFormula L codeF codeR f).
-clear f.
-intros.
-unfold codeFreeVarFormula at 1 in |- *.
-fold g in |- *.
-unfold evalStrongRec in |- *.
-unfold evalComposeFunc in |- *.
-unfold evalOneParamList in |- *.
-rewrite computeEvalStrongRecHelp.
-unfold evalComposeFunc in |- *.
-unfold compose2 in |- *.
-unfold evalList in |- *.
-unfold pred in |- *.
-repeat rewrite cPairProjections1 || rewrite cPairProjections2.
-unfold g at 1 in |- *.
-repeat rewrite cPairProjections1 || rewrite cPairProjections2.
-rewrite (evalStrongRecHelp1 g (cPair 2 n) n).
-simpl in |- *.
-reflexivity.
-apply cPairLt2.
-simpl in |- *.
-rewrite <- codeListRemoveCorrect.
-rewrite <- Hrecf.
-generalize (codeFormula L codeF codeR f).
-clear Hrecf f.
-intros.
-unfold codeFreeVarFormula at 1 in |- *.
-fold g in |- *.
-unfold evalStrongRec in |- *.
-unfold evalComposeFunc in |- *.
-unfold evalOneParamList in |- *.
-unfold evalList in |- *.
-rewrite computeEvalStrongRecHelp.
-unfold evalComposeFunc in |- *.
-unfold compose2 in |- *.
-unfold evalList in |- *.
-unfold pred in |- *.
-repeat rewrite cPairProjections1 || rewrite cPairProjections2.
-unfold g at 1 in |- *.
-repeat rewrite cPairProjections1 || rewrite cPairProjections2.
-rewrite (evalStrongRecHelp1 g (cPair 3 (cPair n n0)) n0).
-simpl in |- *.
-reflexivity.
-eapply Nat.lt_le_trans.
-apply cPairLt2.
-apply cPairLe3.
-apply le_n.
-apply cPairLe2.
+  set
+    (g :=
+       fun f recs : nat =>
+         switchPR (car f)
+           (switchPR (pred (car f))
+              (switchPR (pred (pred (car f)))
+                 (switchPR (pred (pred (pred (car f))))
+                    (codeFreeVarTerms (cdr f))
+                    (codeListRemove (car (cdr f))
+                       (codeNth (f - S (cdr (cdr f))) recs)))
+                 (codeNth (f - S (cdr f)) recs))
+              (codeApp (codeNth (f - S (car (cdr f))) recs)
+                 (codeNth (f - S (cdr (cdr f))) recs)))
+           (codeApp (codeFreeVarTerm (car (cdr f)))
+              (codeFreeVarTerm (cdr (cdr f))))) 
+    in *.
+  induction f as [t t0| r t| f1 Hrecf1 f0 Hrecf0| f Hrecf| n f Hrecf].
+  - simpl; rewrite <- codeAppCorrect; repeat rewrite <- codeFreeVarTermCorrect.
+    generalize (codeTerm L codeF t) (codeTerm L codeF t0).
+    clear t t0; intros n n0. 
+    unfold codeFreeVarFormula, evalStrongRec; simpl.
+    repeat rewrite cPairProjections1 || rewrite cPairProjections2.
+    simpl; reflexivity.
+  - simpl; rewrite <- codeFreeVarTermsCorrect.
+    generalize (codeTerms L codeF (arity L (inl (Functions L) r)) t).
+    clear t.
+    intros n; unfold codeFreeVarFormula, evalStrongRec.
+    unfold evalStrongRecHelp, evalComposeFunc, evalOneParamList, 
+      evalPrimRecFunc.
+    repeat rewrite cPairProjections1 || rewrite cPairProjections2.
+    simpl; repeat rewrite cPairProjections1 || rewrite cPairProjections2.
+    reflexivity.
+  - simpl; rewrite <- codeAppCorrect.
+    rewrite <- Hrecf1.
+    rewrite <- Hrecf0.
+    clear Hrecf0 Hrecf1.
+    unfold codeFreeVarFormula; fold g; unfold evalStrongRec. 
+    unfold evalComposeFunc, evalOneParamList.
+    rewrite computeEvalStrongRecHelp.
+    simpl in |- *.
+    repeat rewrite cPairProjections1 || rewrite cPairProjections2.
+    unfold g at 1 in |- *.
+    repeat rewrite cPairProjections1 || rewrite cPairProjections2.
+    rewrite
+      (evalStrongRecHelp1 g
+         (cPair 1
+            (cPair (codeFormula L codeF codeR f1) 
+               (codeFormula L codeF codeR f0)))
+         (codeFormula L codeF codeR f1)).
+    + rewrite
+        (evalStrongRecHelp1 g
+           (cPair 1
+              (cPair (codeFormula L codeF codeR f1)
+                 (codeFormula L codeF codeR f0)))
+           (codeFormula L codeF codeR f0)).
+      * simpl; unfold evalStrongRec, evalComposeFunc, evalOneParamList.
+        simpl; repeat rewrite cPairProjections1 || rewrite cPairProjections2.
+        reflexivity.
+      * eapply Nat.lt_le_trans.
+        -- apply cPairLt2.
+        -- apply cPairLe3.
+           ++ apply le_n.
+           ++ apply cPairLe2.
+    + eapply Nat.lt_le_trans.
+      * apply cPairLt2.
+      * apply cPairLe3.
+        -- apply le_n.
+        -- apply cPairLe1.
+  - simpl; rewrite <- Hrecf; clear Hrecf.
+    generalize (codeFormula L codeF codeR f).
+    clear f.
+    intros n; unfold codeFreeVarFormula at 1; fold g.
+    unfold evalStrongRec, evalComposeFunc, evalOneParamList.
+    rewrite computeEvalStrongRecHelp; unfold evalComposeFunc, compose2.
+    unfold evalList, pred;
+      repeat rewrite cPairProjections1 || rewrite cPairProjections2.
+    unfold g at 1; repeat rewrite cPairProjections1 || rewrite cPairProjections2.
+    rewrite (evalStrongRecHelp1 g (cPair 2 n) n).
+    simpl; reflexivity.
+    apply cPairLt2; simpl. 
+  - simpl; rewrite <- codeListRemoveCorrect.
+    rewrite <- Hrecf; generalize (codeFormula L codeF codeR f).
+    clear Hrecf f; intros n0.
+    unfold codeFreeVarFormula at 1; fold g; unfold evalStrongRec.
+    unfold evalComposeFunc, evalOneParamList, evalList.
+    rewrite computeEvalStrongRecHelp.
+    unfold evalComposeFunc, compose2, evalList, pred.  
+    repeat rewrite cPairProjections1 || rewrite cPairProjections2.
+    unfold g at 1; 
+      repeat rewrite cPairProjections1 || rewrite cPairProjections2.
+    rewrite (evalStrongRecHelp1 g (cPair 3 (cPair n n0)) n0).
+    + simpl; reflexivity.
+    + eapply Nat.lt_le_trans.
+      * apply cPairLt2.
+      * apply cPairLe3.
+        -- apply le_n.
+        -- apply cPairLe2.
 Qed.
 
 Lemma codeFreeVarFormulaIsPR : isPR 1 codeFreeVarFormula.
 Proof.
-unfold codeFreeVarFormula in |- *.
-apply evalStrongRecIsPR.
-assert (isPR 1 (fun x : nat => pred (cPairPi1 x))).
-apply compose1_1IsPR.
-apply cPairPi1IsPR.
-apply predIsPR.
-assert (isPR 1 (fun x : nat => pred (pred (cPairPi1 x)))).
-apply compose1_1IsPR with (f := fun x : nat => pred (cPairPi1 x)).
-auto.
-apply predIsPR.
-assert (isPR 1 (fun x : nat => pred (pred (pred (cPairPi1 x))))).
-apply compose1_1IsPR with (f := fun x : nat => pred (pred (cPairPi1 x))).
-auto.
-apply predIsPR.
-apply
- compose2_3IsPR
-  with
-    (f1 := fun f recs : nat => cPairPi1 f)
+  unfold codeFreeVarFormula; apply evalStrongRecIsPR.
+  assert (H: isPR 1 (fun x : nat => pred (car x))).
+  { apply compose1_1IsPR.
+    - apply cPairPi1IsPR.
+    - apply predIsPR.
+  } 
+  assert (H0: isPR 1 (fun x : nat => pred (pred (car x)))).
+  { 
+    apply compose1_1IsPR with (f := fun x : nat => pred (car x)).
+    apply H. 
+    apply predIsPR.
+  } 
+  assert (H1: isPR 1 (fun x : nat => pred (pred (pred (car x))))).
+  { apply compose1_1IsPR with 
+      (f := fun x : nat => pred (pred (car x))).
+    apply H0. 
+    apply predIsPR.
+  } 
+  apply compose2_3IsPR with
+    (f1 := fun f recs : nat => car f)
     (f2 := fun f recs : nat =>
-           switchPR (pred (cPairPi1 f))
-             (switchPR (pred (pred (cPairPi1 f)))
-                (switchPR (pred (pred (pred (cPairPi1 f))))
-                   (codeFreeVarTerms (cPairPi2 f))
-                   (codeListRemove (cPairPi1 (cPairPi2 f))
-                      (codeNth (f - S (cPairPi2 (cPairPi2 f))) recs)))
-                (codeNth (f - S (cPairPi2 f)) recs))
-             (codeApp (codeNth (f - S (cPairPi1 (cPairPi2 f))) recs)
-                (codeNth (f - S (cPairPi2 (cPairPi2 f))) recs)))
+             switchPR (pred (car f))
+               (switchPR (pred (pred (car f)))
+                  (switchPR (pred (pred (pred (car f))))
+                     (codeFreeVarTerms (cdr f))
+                     (codeListRemove (car (cdr f))
+                        (codeNth (f - S (cdr (cdr f))) recs)))
+                  (codeNth (f - S (cdr f)) recs))
+               (codeApp (codeNth (f - S (car (cdr f))) recs)
+                  (codeNth (f - S (cdr (cdr f))) recs)))
     (f3 := fun f recs : nat =>
-           codeApp (codeFreeVarTerm (cPairPi1 (cPairPi2 f)))
-             (codeFreeVarTerm (cPairPi2 (cPairPi2 f)))).
-apply filter10IsPR.
-apply cPairPi1IsPR.
-apply
- compose2_3IsPR
-  with
-    (f1 := fun f recs : nat => pred (cPairPi1 f))
-    (f2 := fun f recs : nat =>
-           switchPR (pred (pred (cPairPi1 f)))
-             (switchPR (pred (pred (pred (cPairPi1 f))))
-                (codeFreeVarTerms (cPairPi2 f))
-                (codeListRemove (cPairPi1 (cPairPi2 f))
-                   (codeNth (f - S (cPairPi2 (cPairPi2 f))) recs)))
-             (codeNth (f - S (cPairPi2 f)) recs))
-    (f3 := fun f recs : nat =>
-           codeApp (codeNth (f - S (cPairPi1 (cPairPi2 f))) recs)
-             (codeNth (f - S (cPairPi2 (cPairPi2 f))) recs)).
-apply filter10IsPR with (g := fun x : nat => pred (cPairPi1 x)).
-auto.
-apply
- compose2_3IsPR
-  with
-    (f1 := fun f recs : nat => pred (pred (cPairPi1 f)))
-    (f2 := fun f recs : nat =>
-           switchPR (pred (pred (pred (cPairPi1 f))))
-             (codeFreeVarTerms (cPairPi2 f))
-             (codeListRemove (cPairPi1 (cPairPi2 f))
-                (codeNth (f - S (cPairPi2 (cPairPi2 f))) recs)))
-    (f3 := fun f recs : nat => codeNth (f - S (cPairPi2 f)) recs).
-apply filter10IsPR with (g := fun x : nat => pred (pred (cPairPi1 x))).
-auto.
-apply
- compose2_3IsPR
-  with
-    (f1 := fun f recs : nat => pred (pred (pred (cPairPi1 f))))
-    (f2 := fun f recs : nat => codeFreeVarTerms (cPairPi2 f))
-    (f3 := fun f recs : nat =>
-           codeListRemove (cPairPi1 (cPairPi2 f))
-             (codeNth (f - S (cPairPi2 (cPairPi2 f))) recs)).
-apply filter10IsPR with (g := fun x : nat => pred (pred (pred (cPairPi1 x)))).
-auto.
-apply filter10IsPR with (g := fun f : nat => codeFreeVarTerms (cPairPi2 f)).
-apply compose1_1IsPR.
-apply cPairPi2IsPR.
-apply codeFreeVarTermsIsPR.
-apply
- compose2_2IsPR
-  with
-    (f := fun f recs : nat => cPairPi1 (cPairPi2 f))
-    (g := fun f recs : nat => codeNth (f - S (cPairPi2 (cPairPi2 f))) recs).
-apply filter10IsPR with (g := fun f : nat => cPairPi1 (cPairPi2 f)).
-apply compose1_1IsPR.
-apply cPairPi2IsPR.
-apply cPairPi1IsPR.
-apply
- compose2_2IsPR
-  with
-    (f := fun f recs : nat => f - S (cPairPi2 (cPairPi2 f)))
-    (g := fun f recs : nat => recs).
-apply filter10IsPR with (g := fun f : nat => f - S (cPairPi2 (cPairPi2 f))).
-apply
- compose1_2IsPR
-  with
-    (f := fun f : nat => f)
-    (f' := fun f : nat => S (cPairPi2 (cPairPi2 f))).
-apply idIsPR.
-apply compose1_1IsPR with (f := fun f : nat => cPairPi2 (cPairPi2 f)).
-apply compose1_1IsPR; apply cPairPi2IsPR.
-apply succIsPR.
-apply minusIsPR.
-apply pi2_2IsPR.
-apply codeNthIsPR.
-apply codeListRemoveIsPR.
-apply switchIsPR.
-apply
- compose2_2IsPR
-  with
-    (f := fun f recs : nat => f - S (cPairPi2 f))
-    (g := fun f recs : nat => recs).
-apply filter10IsPR with (g := fun f : nat => f - S (cPairPi2 f)).
-apply
- compose1_2IsPR
-  with (f := fun f : nat => f) (f' := fun f : nat => S (cPairPi2 f)).
-apply idIsPR.
-apply compose1_1IsPR.
-apply cPairPi2IsPR.
-apply succIsPR.
-apply minusIsPR.
-apply pi2_2IsPR.
-apply codeNthIsPR.
-apply switchIsPR.
-apply
- compose2_2IsPR
-  with
-    (f := fun f recs : nat => codeNth (f - S (cPairPi1 (cPairPi2 f))) recs)
-    (g := fun f recs : nat => codeNth (f - S (cPairPi2 (cPairPi2 f))) recs).
-apply
- compose2_2IsPR
-  with
-    (f := fun f recs : nat => f - S (cPairPi1 (cPairPi2 f)))
-    (g := fun f recs : nat => recs).
-apply filter10IsPR with (g := fun f : nat => f - S (cPairPi1 (cPairPi2 f))).
-apply
- compose1_2IsPR
-  with
-    (f := fun f : nat => f)
-    (f' := fun f : nat => S (cPairPi1 (cPairPi2 f))).
-apply idIsPR.
-apply compose1_1IsPR with (f := fun f : nat => cPairPi1 (cPairPi2 f)).
-apply compose1_1IsPR.
-apply cPairPi2IsPR.
-apply cPairPi1IsPR.
-apply succIsPR.
-apply minusIsPR.
-apply pi2_2IsPR.
-apply codeNthIsPR.
-apply
- compose2_2IsPR
-  with
-    (f := fun f recs : nat => f - S (cPairPi2 (cPairPi2 f)))
-    (g := fun f recs : nat => recs).
-apply filter10IsPR with (g := fun f : nat => f - S (cPairPi2 (cPairPi2 f))).
-apply
- compose1_2IsPR
-  with
-    (f := fun f : nat => f)
-    (f' := fun f : nat => S (cPairPi2 (cPairPi2 f))).
-apply idIsPR.
-apply compose1_1IsPR with (f := fun f : nat => cPairPi2 (cPairPi2 f)).
-apply compose1_1IsPR; apply cPairPi2IsPR.
-apply succIsPR.
-apply minusIsPR.
-apply pi2_2IsPR.
-apply codeNthIsPR.
-apply codeAppIsPR.
-apply switchIsPR.
-apply
- filter10IsPR
-  with
+             codeApp (codeFreeVarTerm (car (cdr f)))
+               (codeFreeVarTerm (cdr (cdr f)))).
+  - apply filter10IsPR; apply cPairPi1IsPR.
+  - apply compose2_3IsPR with
+      (f1 := fun f recs : nat => pred (car f))
+      (f2 := fun f recs : nat =>
+               switchPR (pred (pred (car f)))
+                 (switchPR (pred (pred (pred (car f))))
+                    (codeFreeVarTerms (cdr f))
+                    (codeListRemove (car (cdr f))
+                       (codeNth (f - S (cdr (cdr f))) recs)))
+                 (codeNth (f - S (cdr f)) recs))
+      (f3 := fun f recs : nat =>
+               codeApp (codeNth (f - S (car (cdr f))) recs)
+                 (codeNth (f - S (cdr (cdr f))) recs)).
+    + apply filter10IsPR with (g := fun x : nat => pred (car x)), H.
+    + apply compose2_3IsPR with
+        (f1 := fun f recs : nat => pred (pred (car f)))
+        (f2 := fun f recs : nat =>
+                 switchPR (pred (pred (pred (car f))))
+                   (codeFreeVarTerms (cdr f))
+                   (codeListRemove (car (cdr f))
+                      (codeNth (f - S (cdr (cdr f))) recs)))
+        (f3 := fun f recs : nat => codeNth (f - S (cdr f)) recs).
+      * apply filter10IsPR with 
+          (g := fun x : nat => pred (pred (car x))), H0.
+      * apply compose2_3IsPR with
+          (f1 := fun f recs : nat => pred (pred (pred (car f))))
+          (f2 := fun f recs : nat => codeFreeVarTerms (cdr f))
+          (f3 := fun f recs : nat =>
+                   codeListRemove (car (cdr f))
+                     (codeNth (f - S (cdr (cdr f))) recs)).
+      -- apply filter10IsPR with 
+           (g := fun x : nat => pred (pred (pred (car x)))), H1.
+      -- apply filter10IsPR with 
+           (g := fun f : nat => codeFreeVarTerms (cdr f)).
+         apply compose1_1IsPR.
+         ++ apply cPairPi2IsPR.
+         ++ apply codeFreeVarTermsIsPR.
+      -- apply compose2_2IsPR with
+           (f := fun f recs : nat => car (cdr f))
+           (g := fun f recs : nat => codeNth 
+                                       (f - S (cddr f)) recs).
+         ++ apply filter10IsPR with (g := fun f : nat => car (cdr f)).
+            apply compose1_1IsPR.
+            apply cPairPi2IsPR.
+            apply cPairPi1IsPR.
+         ++ apply compose2_2IsPR with
+              (f := fun f recs : nat => f - S (cddr f))
+              (g := fun f recs : nat => recs).
+            apply filter10IsPR with (g := fun f : nat => f - S (cddr f)).
+            apply compose1_2IsPR with
+              (f := fun f : nat => f)
+              (f' := fun f : nat => S (cddr f)).
+            apply idIsPR.
+            apply compose1_1IsPR with (f := fun f : nat => cddr f).
+            apply compose1_1IsPR; apply cPairPi2IsPR.
+            apply succIsPR.
+            apply minusIsPR.
+            apply pi2_2IsPR.
+            apply codeNthIsPR.
+         ++ apply codeListRemoveIsPR.
+      -- apply switchIsPR.
+      * apply compose2_2IsPR with
+          (f := fun f recs : nat => f - S (cdr f))
+          (g := fun f recs : nat => recs).
+        -- apply filter10IsPR with (g := fun f : nat => f - S (cdr f)).
+           apply compose1_2IsPR with 
+             (f := fun f : nat => f) 
+             (f' := fun f : nat => S (cdr f)).
+           ++ apply idIsPR.
+           ++ apply compose1_1IsPR.
+              ** apply cPairPi2IsPR.
+              ** apply succIsPR.
+           ++ apply minusIsPR.
+        -- apply pi2_2IsPR.
+        -- apply codeNthIsPR.
+      * apply switchIsPR.
+    + apply compose2_2IsPR with
+        (f := fun f recs : nat => codeNth (f - S (car (cdr f))) recs)
+        (g := fun f recs : nat => codeNth (f - S (cddr f)) recs).
+      * apply compose2_2IsPR with
+          (f := fun f recs : nat => f - S (car (cdr f)))
+          (g := fun f recs : nat => recs).
+        apply filter10IsPR with (g := fun f : nat => f - S (car (cdr f))).
+        -- apply compose1_2IsPR with
+             (f := fun f : nat => f)
+             (f' := fun f : nat => S (car (cdr f))).
+           ++ apply idIsPR.
+           ++ apply compose1_1IsPR with 
+                (f := fun f : nat => car (cdr f)).
+              ** apply compose1_1IsPR.
+                 apply cPairPi2IsPR.
+                 apply cPairPi1IsPR.
+              ** apply succIsPR.
+           ++ apply minusIsPR.
+        -- apply pi2_2IsPR.
+        -- apply codeNthIsPR.
+      * apply compose2_2IsPR with
+          (f := fun f recs : nat => f - S (cddr f))
+          (g := fun f recs : nat => recs).
+        -- apply filter10IsPR with
+             (g := fun f : nat => f - S (cddr f)).
+           apply  compose1_2IsPR with
+             (f := fun f : nat => f)
+             (f' := fun f : nat => S (cddr f)).
+           ++ apply idIsPR.
+           ++ apply compose1_1IsPR with 
+                (f := fun f : nat => cddr f).
+              ** apply compose1_1IsPR; apply cPairPi2IsPR.
+              ** apply succIsPR.
+           ++ apply minusIsPR.
+        -- apply pi2_2IsPR.
+        -- apply codeNthIsPR.
+      * apply codeAppIsPR.
+    + apply switchIsPR.
+  - apply filter10IsPR  with
     (g := fun f : nat =>
-          codeApp (codeFreeVarTerm (cPairPi1 (cPairPi2 f)))
-            (codeFreeVarTerm (cPairPi2 (cPairPi2 f)))).
-apply
- compose1_2IsPR
-  with
-    (f := fun f : nat => codeFreeVarTerm (cPairPi1 (cPairPi2 f)))
-    (f' := fun f : nat => codeFreeVarTerm (cPairPi2 (cPairPi2 f))).
-apply compose1_1IsPR with (f := fun f : nat => cPairPi1 (cPairPi2 f)).
-apply compose1_1IsPR.
-apply cPairPi2IsPR.
-apply cPairPi1IsPR.
-apply codeFreeVarTermIsPR.
-apply compose1_1IsPR with (f := fun f : nat => cPairPi2 (cPairPi2 f)).
-apply compose1_1IsPR; apply cPairPi2IsPR.
-apply codeFreeVarTermIsPR.
-apply codeAppIsPR.
-apply switchIsPR.
+          codeApp (codeFreeVarTerm (car (cdr f)))
+            (codeFreeVarTerm (cddr f))).
+    apply compose1_2IsPR with
+      (f := fun f : nat => codeFreeVarTerm (car (cdr f)))
+      (f' := fun f : nat => codeFreeVarTerm (cddr f)).
+    + apply compose1_1IsPR with (f := fun f : nat => car (cdr f)).
+      * apply compose1_1IsPR.
+        -- apply cPairPi2IsPR.
+        -- apply cPairPi1IsPR.
+      * apply codeFreeVarTermIsPR.
+    + apply compose1_1IsPR with (f := fun f : nat => cddr f).
+      * apply compose1_1IsPR; apply cPairPi2IsPR.
+      * apply codeFreeVarTermIsPR.
+    + apply codeAppIsPR.
+  - apply switchIsPR.
 Qed.
 
 Definition codeFreeVarListFormula : nat -> nat :=
   evalStrongRec 0
     (fun l recs : nat =>
      switchPR l
-       (codeApp (codeFreeVarFormula (cPairPi1 (pred l)))
-          (codeNth (l - S (cPairPi2 (pred l))) recs)) 0).
+       (codeApp (codeFreeVarFormula (car (pred l)))
+          (codeNth (l - S (cdr (pred l))) recs)) 0).
 
-Lemma codeFreeVarListFormulaCorrect :
- forall l : list Formula,
+Lemma codeFreeVarListFormulaCorrect (l : list Formula):
  codeFreeVarListFormula (codeList (map (codeFormula L codeF codeR) l)) =
  codeList (freeVarListFormula L l).
 Proof.
-intros.
-unfold codeFreeVarListFormula in |- *.
-set
- (A :=
-  fun l0 recs : nat =>
-  switchPR l0
-    (codeApp (codeFreeVarFormula (cPairPi1 (pred l0)))
-       (codeNth (l0 - S (cPairPi2 (pred l0))) recs)) 0) 
- in *.
-induction l as [| a l Hrecl];
- unfold evalStrongRec, evalComposeFunc, evalOneParamList, evalList in |- *;
- rewrite computeEvalStrongRecHelp;
- unfold compose2, evalComposeFunc, evalOneParamList, evalList in |- *.
-simpl in |- *.
-rewrite cPairProjections1.
-reflexivity.
-unfold A at 1 in |- *.
-rewrite evalStrongRecHelp1.
-simpl in |- *.
-repeat first [ rewrite cPairProjections1 | rewrite cPairProjections2 ].
-rewrite Hrecl.
-rewrite codeFreeVarFormulaCorrect.
-apply codeAppCorrect.
-simpl in |- *.
-apply Compat815.le_lt_n_Sm.
-apply cPairLe2A.
+  unfold codeFreeVarListFormula;
+    set
+      (A :=
+         fun l0 recs : nat =>
+           switchPR l0
+             (codeApp (codeFreeVarFormula (car (pred l0)))
+                (codeNth (l0 - S (cdr (pred l0))) recs)) 0) 
+    in *.
+  induction l as [| a l Hrecl];
+    unfold evalStrongRec, evalComposeFunc, evalOneParamList, evalList in |- *;
+    rewrite computeEvalStrongRecHelp;
+    unfold compose2, evalComposeFunc, evalOneParamList, evalList in |- *.
+  - simpl; rewrite cPairProjections1; reflexivity.
+  - unfold A at 1; rewrite evalStrongRecHelp1; simpl. 
+    + repeat first [ rewrite cPairProjections1 | rewrite cPairProjections2 ].
+      rewrite Hrecl, codeFreeVarFormulaCorrect.
+      apply codeAppCorrect.
+    + apply Compat815.le_lt_n_Sm, cPairLe2A.
 Qed.
 
 Lemma codeFreeVarListFormulaIsPR : isPR 1 codeFreeVarListFormula.
 Proof.
-unfold codeFreeVarListFormula in |- *.
-apply evalStrongRecIsPR.
-apply
- compose2_3IsPR
-  with
+  unfold codeFreeVarListFormula; apply evalStrongRecIsPR.
+  apply compose2_3IsPR with
     (f1 := fun l recs : nat => l)
     (f2 := fun l recs : nat =>
-           codeApp (codeFreeVarFormula (cPairPi1 (pred l)))
-             (codeNth (l - S (cPairPi2 (pred l))) recs))
+             codeApp (codeFreeVarFormula (car (pred l)))
+               (codeNth (l - S (cdr (pred l))) recs))
     (f3 := fun l recs : nat => 0).
-apply pi1_2IsPR.
-apply
- compose2_2IsPR
-  with
-    (f := fun l recs : nat => codeFreeVarFormula (cPairPi1 (pred l)))
-    (g := fun l recs : nat => codeNth (l - S (cPairPi2 (pred l))) recs).
-apply
- filter10IsPR
-  with (g := fun l : nat => codeFreeVarFormula (cPairPi1 (pred l))).
-apply compose1_1IsPR with (f := fun l : nat => cPairPi1 (pred l)).
-apply compose1_1IsPR.
-apply predIsPR.
-apply cPairPi1IsPR.
-apply codeFreeVarFormulaIsPR.
-apply callIsPR with (g := fun l : nat => cPairPi2 (pred l)).
-apply compose1_1IsPR.
-apply predIsPR.
-apply cPairPi2IsPR.
-apply codeAppIsPR.
-apply filter10IsPR with (g := fun _ : nat => 0).
-apply const1_NIsPR.
-apply switchIsPR.
+  - apply pi1_2IsPR.
+  - apply compose2_2IsPR with
+    (f := fun l recs : nat => codeFreeVarFormula (car (pred l)))
+    (g := fun l recs : nat => codeNth (l - S (cdr (pred l))) recs).
+    + apply filter10IsPR with
+        (g := fun l : nat => codeFreeVarFormula (car (pred l))).
+      apply compose1_1IsPR with (f := fun l : nat => car (pred l)).
+      * apply compose1_1IsPR.
+        -- apply predIsPR.
+        -- apply cPairPi1IsPR.
+      * apply codeFreeVarFormulaIsPR.
+    + apply callIsPR with (g := fun l : nat => cdr (pred l)).
+      apply compose1_1IsPR.
+      * apply predIsPR.
+      * apply cPairPi2IsPR.
+    + apply codeAppIsPR.
+  - apply filter10IsPR with (g := fun _ : nat => 0), const1_NIsPR.
+  - apply switchIsPR.
 Qed.
 
 End Code_Free_Vars.
